coq/CN_Lemmas/CN_Lib.v
@@ -2,6 +2,140 @@ Require List.
 Require Import ZArith Bool.
 Require Import Lia.
 Require NArith.
+Require Fin.
+Require Import Vector.
+
+Open Scope Z.
+
+(* Bounds on the unsigned integer types. *)
+Notation min_UChar  := 0%Z.
+Notation max_UChar  := (2 ^ 8 - 1)%Z.
+Notation min_UShort := 0%Z.
+Notation max_UShort := (2 ^ 16 - 1)%Z.
+Notation min_UInt   := 0%Z.
+Notation max_UInt   := (2 ^ 32 - 1)%Z.
+Notation min_ULong  := 0%Z.
+Notation max_ULong  := (2 ^ 64 - 1)%Z.
+
+(* Bounds on the signed integer types. *)
+Notation min_Char  := (- (2 ^ 7))%Z.
+Notation max_Char  := (2 ^ 7 - 1)%Z.
+Notation min_Short := (- (2 ^ 15))%Z.
+Notation max_Short := (2 ^ 15 - 1)%Z.
+Notation min_Int   := (- (2 ^ 31))%Z.
+Notation max_Int   := (2 ^ 31 - 1)%Z.
+Notation min_Long  := (- (2 ^ 63))%Z.
+Notation max_Long  := (2 ^ 63 - 1)%Z.
+
+Fixpoint list_of_fin (n : nat) : list (Fin.t n) :=
+  match n with
+  | 0%nat => List.nil
+  | S n' => Fin.F1 :: List.map Fin.FS (list_of_fin n')
+  end.
+
+Fixpoint to_CN_Bytes (n : nat) (v : Z) : (Vector.t Z n) :=
+  match n with
+  | O => Vector.nil Z
+  | S n' => Vector.cons Z (v mod 256) n' (to_CN_Bytes n' (v / 256))
+  end.
+
+Definition from_CN_Bytes {n : nat} (v : Vector.t Z n) : Z :=
+List.fold_left
+  (fun acc i =>
+      acc + nth v i * 2 ^ (8 * Z.of_nat (proj1_sig(Fin.to_nat i))))
+  (list_of_fin n)
+  0.
+
+
+Definition UShort_bytes (v : Z) : Vector.t Z 2 := to_CN_Bytes 2 v.
+Definition UInt_bytes   (v : Z) : Vector.t Z 4 := to_CN_Bytes 4 v.
+Definition ULong_bytes  (v : Z) : Vector.t Z 8 := to_CN_Bytes 8 v.
+
+Theorem UShort_idem {v : Z} :
+   min_UShort <= v /\ v <= max_UShort
+  -> v = from_CN_Bytes (UShort_bytes v).
+Proof.
+  intros (H1, H2); unfold max_UShort in H2; simpl in H2.
+  unfold from_CN_Bytes, UShort_bytes; cbn.
+  assert (Hv : v = 256 * (v / 256) + v mod 256) by (apply Z.div_mod; lia).
+  assert (Hv'' : 0 <= v / 256 < 256).
+    { constructor.
+    - apply Z.div_le_lower_bound; lia.
+    - apply Z.div_lt_upper_bound; lia. }
+  rewrite Z.mul_1_r, Z.mul_comm, Z.add_comm, Hv at 1.
+  do 2 f_equal.
+  rewrite Z.mod_small; auto.
+Qed.
+
+Theorem UInt_idem {v : Z} :
+   min_UInt <= v /\ v <= max_UInt
+  -> v = from_CN_Bytes (UInt_bytes v).
+Proof.
+  intros (H1, H2); unfold max_UInt in H2; simpl in H2.
+  unfold from_CN_Bytes, UInt_bytes; cbn.
+  rewrite Z.mul_1_r, Z.mul_comm, Z.add_comm. 
+  (* First division *)
+  assert (H3 : v = 256 * (v / 256) + v mod 256) by (apply Z.div_mod; lia).
+  (* Second division *)
+  assert (H4 : v / 256 = 256 * (v / 256 / 256) + (v / 256) mod 256) by (apply Z.div_mod; lia).
+  (* Third division *)
+  assert (H5 : v / 256 / 256 = 256 * (v / 256 / 256 / 256) +
+      (v / 256 / 256) mod 256)  by (apply Z.div_mod; lia).
+  (* max bound *)
+  assert (H6 :
+    v / 256 / 256 / 256 < 256).
+  { repeat (apply Z.div_lt_upper_bound; [lia |]).
+    lia. }
+  (* min bound *)
+  assert (H7 : 
+    0 <= v / 256 / 256 / 256 < 256).
+  { constructor.
+    - repeat (apply Z.div_le_lower_bound; [lia; simpl |]); lia.
+    - repeat (apply Z.div_lt_upper_bound; [lia; simpl |]); lia. }
+  assert (H4mod :
+    (v / 256 / 256 / 256) mod 256 = v / 256 / 256 / 256) by (apply Z.mod_small; lia).
+  rewrite H4mod.
+  rewrite H3 at 1.
+  rewrite H4 at 1.
+  rewrite H5 at 1.
+  lia.
+Qed.
+
+(* TODO: Prove the above theorem for ULong *)
+
+Theorem UShort_eq {v v' : Z} :
+    min_UShort <= v /\ v <= max_UShort
+  -> min_UShort <= v' /\ v' <= max_UShort
+  -> UShort_bytes v = UShort_bytes v'
+  -> v = v'.
+Proof.
+  intros Hv Hv' H.
+  unfold UShort_bytes in H.
+  assert (HEq : v = from_CN_Bytes (UShort_bytes v)) by (apply UShort_idem; assumption).
+  assert (HEq' : v' = from_CN_Bytes (UShort_bytes v')) by (apply UShort_idem; assumption).
+  unfold UShort_bytes in HEq, HEq'.
+  rewrite H in HEq.
+  rewrite <- HEq' in HEq.
+  assumption.
+Qed.
+
+Theorem UInt_eq {v v' : Z} :
+    min_UInt <= v /\ v <= max_UInt
+  -> min_UInt <= v' /\ v' <= max_UInt
+  -> UInt_bytes v = UInt_bytes v'
+  -> v = v'.
+Proof.
+  intros Hv Hv' H.
+  unfold UInt_bytes in H.
+  assert (HEq : v = from_CN_Bytes (UInt_bytes v)) by (apply UInt_idem; assumption).
+  assert (HEq' : v' = from_CN_Bytes (UInt_bytes v')) by (apply UInt_idem; assumption).
+  unfold UInt_bytes in HEq, HEq'.
+  rewrite H in HEq.
+  rewrite <- HEq' in HEq. 
+  assumption.
+Qed.
+
+(* TODO: Prove the above theorem for ULong *)
 
 Definition wrapI (minInt : Z) (maxInt : Z) x :=
   let delta := ((maxInt - minInt) + 1)%Z in
@@ -27,3 +161,12 @@ Proof.
     + lia.
     + exists (-1); lia.
 Qed.
+
+(* TODO: Prove this theorem *)
+Theorem wrapI_within_bounds :
+  forall {min max x : Z}, (min <= 0 /\ 0 < max) ->
+  min <= wrapI min max x /\ wrapI min max x <= max.
+Proof.
+  Admitted.
+
+(* TODO: Prove the rest of the `wrapI_*` theorems from the Lean library *)
